\documentclass{article}
\usepackage{amsmath}
\begin{document}
	\begin{minipage}{0.5\textwidth}
		\begin{align*}
			&x=\frac{-b\pm\sqrt{b^{2}-4ac}}{2a}\\
			&=\frac{-2\pm\sqrt{2^2-4*(1)*1(-8)}}{2*1}\\
			&=\frac{-2\pm\sqrt{4+32}}{2}
		\end{align*}
	\end{minipage}
	\hfill
   \begin{minipage}{0.5\textwidth}
     \begin{align*}
		 \varphi_\sigma^{\lambda}A_t &=\sum_{\pi\epsilon c_{t}}  \operatorname{sgn}(\pi)\varphi_\sigma^{\lambda}\varphi_\pi^{\lambda}\\
		 &= \sum_{\tau\epsilon C_{\sigma t}} \operatorname{sgn}(\sigma^{-1}\tau\sigma)\varphi_\sigma^{\lambda}\varphi_{\sigma^{-1}{\sigma}}^{\lambda}\\
		 &=\operatorname{A}_\sigma\operatorname{t}\varphi_\sigma^{\lambda}
	 \end{align*}
  \end{minipage}
\end{document}
	